src/Spec/Abstraction.v
@@ -1,0 +1,88 @@
+Require Import ConcurProc.
+Require Import Relations.Relation_Operators.
+Require Import RelationClasses.
+Require Import Morphisms.
+Require Import Helpers.Helpers.
+Require Import Helpers.ListStuff.
+Require Import List.
+Require Import Omega.
+
+Import ListNotations.
+
+Global Set Implicit Arguments.
+Global Generalizable All Variables.
+
+
+(** Inclusion of traces across state abstraction *)
+
+Section StateAbstraction.
+
+  Variable opLoT : Type -> Type.
+  Variable opHiT : Type -> Type.
+
+  Variable StateLo : Type.
+  Variable StateHi : Type.
+  Variable absR : StateLo -> StateHi -> Prop.
+
+  Variable lo_step : OpSemantics opLoT StateLo.
+  Variable hi_step : OpSemantics opLoT StateHi.
+
+  Definition op_abs := forall `(op : opLoT T) s1 s1' s2 tid r,
+    absR s1 s2 ->
+    lo_step op tid s1 r s1' ->
+      exists s2',
+        absR s1' s2' /\
+        hi_step op tid s2 r s2'.
+
+  Variable op_abs_holds : op_abs.
+
+  Theorem atomic_exec_abs : forall `(p : proc opLoT opHiT T) s1 s1' s2 tid r evs,
+    absR s1 s2 ->
+    atomic_exec lo_step p tid s1 r s1' evs ->
+      exists s2',
+        absR s1' s2' /\
+        atomic_exec hi_step p tid s2 r s2' evs.
+  Proof.
+    intros.
+    generalize dependent s2.
+    induction H0; intros.
+    all: try solve [ eexists; eauto ].
+    - edestruct IHatomic_exec1; intuition eauto.
+      edestruct IHatomic_exec2; intuition eauto.
+    - eapply op_abs_holds in H; eauto; deex.
+      eexists; eauto.
+    - edestruct IHatomic_exec; intuition eauto.
+  Qed.
+
+  Theorem exec_tid_abs : forall `(p : proc opLoT opHiT T) s1 s1' s2 tid res evs,
+    absR s1 s2 ->
+    exec_tid lo_step tid s1 p s1' res evs ->
+      exists s2',
+        absR s1' s2' /\
+        exec_tid hi_step tid s2 p s2' res evs.
+  Proof.
+    intros.
+    induction H0.
+    all: try solve [ eexists; eauto ].
+    - eapply op_abs_holds in H0; eauto; deex.
+      eexists; eauto.
+    - eapply atomic_exec_abs in H0; eauto; deex.
+      eexists; eauto.
+    - destruct IHexec_tid; intuition eauto.
+  Qed.
+
+  Theorem trace_incl_abs :
+    forall s1 s2 (ts : @threads_state opLoT opHiT) tr,
+      absR s1 s2 ->
+      exec lo_step s1 ts tr ->
+      exec hi_step s2 ts tr.
+  Proof.
+    intros.
+    generalize dependent s2.
+    induction H0; intros.
+    - eapply exec_tid_abs in H0; eauto; deex.
+      eapply ExecOne with (tid := tid); eauto.
+    - eapply ExecEmpty; eauto.
+  Qed.
+
+End StateAbstraction.
